## Problem 1

![alt text](image.png)

### 1.1

This is to prove $F \ \text{logically implies} \ (F \backslash \{X \rightarrow Y\}) \cup \{ X \backslash \{A\} \rightarrow Y \} \Leftrightarrow Y \subseteq (X \backslash \{A\})_F^+$.

$\Rightarrow$:

If $F \ \text{logically implies} \ (F \backslash \{X \rightarrow Y\}) \cup \{ X \backslash \{A\} \rightarrow Y \}$, then $F \ \text{logically implies} \ \{ X \backslash \{A\} \rightarrow Y \}$.

From the definition of the closure of attributes $X \backslash \{A\}$ under $F$, we know that $Y \subseteq (X \backslash \{A\})_F^+$.

$\Leftarrow$:

If $Y \subseteq (X \backslash \{A\})_F^+$, then $F \ \text{logically implies} \ \{ X \backslash \{A\} \rightarrow Y \}$, and we know $F \ \text{logically implies} \ (F \backslash \{X \rightarrow Y\})$, so $F \ \text{logically implies} \ (F \backslash \{X \rightarrow Y\}) \cup \{ X \backslash \{A\} \rightarrow Y \}$.

Thus the lemma is proved.

### 1.2

The lemma 1.2 is to prove 


